made wellformedness of source types a separate judgement

rules_src.v
@@ -3,27 +3,31 @@ Require Import Tactics Sequence source subst_src (*SimpSub*).
 
 Require Import Defined.
 
+
+Inductive typ: term -> Prop :=
+  nattyp : typ nattp_m
+| arrowtyp : forall A1 A2, typ A1 -> typ A2 -> typ (arrow_m A1 A2)
+| reftyp: forall A, typ A -> typ (reftp_m A)
+| comptyp: forall A, typ A -> typ (comp_m A)
+| compunit : typ unittp_m.
+
+
 Inductive of_m : context -> term -> term -> Type :=
 
 (* Hypotheses *)
 
 | of_m_hyp_tm :
     forall G i a,
-      index i G a
-      -> of_m G  (var i) (subst_src.subst (subst_src.sh (S i)) a)
+      typ a ->
+      index i G a ->
+      of_m G  (var i) a
 | of_m_z: forall G, of_m G z_m nattp_m
 | of_m_succ: forall G M,
     of_m G M nattp_m ->
     of_m G  (succ_m M) nattp_m
-| of_m_natform: forall G, of_m G nattp_m typ
-| of_m_arrow_form :
-    forall G a b,
-      of_m G a typ
-      -> of_m G b typ
-      -> of_m G (arrow_m a b) typ
 | of_m_arrow_m_inof_mo :
     forall G a b m,
-      of_m G a typ
+      typ a
       -> of_m (cons a G) m b
       -> of_m G (lam_m m) (arrow_m a b)
 | of_m_arrow_m_elim :
@@ -31,16 +35,14 @@ Inductive of_m : context -> term -> term -> Type :=
       of_m G m (arrow_m a b)
       -> of_m G p a
       -> of_m G (app_m m p) b
-| of_m_comp: forall G A, of_m G A typ -> of_m G (comp_m A) typ
 | of_m_ret: forall G E A, of_m G E A -> of_m G (ret_m E) (comp_m A)
 | of_m_bind: forall G A B V E,
+    typ A ->
     of_m G V (comp_m A) -> 
     of_m (cons A G) E (comp_m B) ->
     of_m G (bind_m V E) (comp_m B)
-|of_m_reftp: forall G A, of_m G A typ -> of_m G (reftp_m A) typ
 | of_m_ref: forall G E A, of_m G E A -> of_m G (ref_m E) (comp_m (reftp_m A))
 | of_m_asgn: forall G R V T, of_m G V T ->
                       of_m G R (comp_m (reftp_m T)) ->
                       of_m G (asgn_m R V) (comp_m unittp_m)
-| of_m_triv: forall G, of_m G triv_m unittp_m
-| of_m_null: forall G, of_m G unittp_m typ.
+| of_m_triv: forall G, of_m G triv_m unittp_m.
