proofs_trans.v
@@ -1,0 +1,26 @@
+Require Import Program Equality Ring Lia Omega.
+From Coq Require Import ssreflect ssrfun ssrbool.
+From mathcomp Require Import seq eqtype ssrnat.
+From istari Require Import lemmas0
+     source subst_src rules_src basic_types0 basic_types
+     help subst_help0 subst_help trans derived_rules embedded_lemmas proofs.
+From istari Require Import Sigma Tactics
+     Syntax Subst SimpSub Promote Hygiene
+     ContextHygiene Equivalence Equivalences.
+From istari Require Import Rules Defined DefsEquiv.
+
+Theorem total G E A: of_m G E A ->
+                exists ebar, trans G E A ebar.
+  intros He. induction He.
+  {exists (lam (lam (gamma_nth (var 0) i))). constructor. assumption.
+  }
+  { exists (lam (lam nzero)). constructor. 
+  }
+  {
+    destruct IHHe as [mbar Hm].
+    exists (lam (lam (app (app (subst (sh 2) mbar) (var 1)) (var 0)))).
+    constructor. assumption.
+  }
+  {
+    (*make separate judgement to tell if a term is a type*)
+  }
